Misc

Object_Model.thy
@@ -41,42 +41,68 @@ definition assoc_refer_role :: "(role \<rightharpoonup>\<^sub>f 'a assoc_end) \<
    С другой стороны, не очень понятно зачем. Для определения типа не нужен,
    нужен для вычисления значения  *)
 
-definition assoc_refer_class :: "(role \<rightharpoonup>\<^sub>f 'a assoc_end) \<Rightarrow> 'a \<Rightarrow> bool" where
-  "assoc_refer_class ends cls \<equiv>
-    fBex (fmdom ends) (\<lambda>role. assoc_end_class (the (fmlookup ends role)) = cls)"
+definition "attrs_ok attrs \<equiv> \<nexists>\<C> \<D> attrs\<^sub>\<C> attrs\<^sub>\<D> attr.
+  \<C> < \<D> \<and>
+  fmlookup attrs \<C> = Some attrs\<^sub>\<C> \<and>
+  fmlookup attrs \<D> = Some attrs\<^sub>\<D> \<and>
+  fmlookup attrs\<^sub>\<C> attr \<noteq> None \<and>
+  fmlookup attrs\<^sub>\<D> attr \<noteq> None"
 
-definition find_assocs :: "'a assocs \<Rightarrow> 'a \<Rightarrow> role \<Rightarrow> 'a assocs" where
-  "find_assocs assocs cls role \<equiv>
-    fmfilter (\<lambda>assoc.
-      case fmlookup assocs assoc of None \<Rightarrow> False | Some ends \<Rightarrow>
-        assoc_refer_class (fmdrop role ends) cls \<and> assoc_refer_role ends role) assocs"
+inductive find_attribute where
+  "\<C> \<le> \<D> \<Longrightarrow>
+   fmlookup attrs \<D> = Some attrs\<^sub>\<D> \<Longrightarrow>
+   fmlookup attrs\<^sub>\<D> attr = Some \<tau> \<Longrightarrow>
+   find_attribute attrs \<C> attr \<D> \<tau>"
 
-definition find_assoc_end :: "'a assocs \<Rightarrow> 'a \<Rightarrow> role \<Rightarrow> 'a assoc_end option" where
-  "find_assoc_end assocs cls role \<equiv>
-    let found = fmran (find_assocs assocs cls role) in
-    if fcard found = 1 then fmlookup (fthe_elem found) role else None"
-
-(*
 inductive find_association where
-  "(*cls \<le> cls2 \<Longrightarrow>*)
-   assoc \<in> fmdom' assocs \<Longrightarrow>
-   fmlookup assocs assoc = Some ends \<Longrightarrow>
-   assoc_refer_class (fmdrop name ends) cls \<Longrightarrow>
-   fmlookup ends name = Some end \<Longrightarrow>
-   find_association (fmupd assoc ends assocs) cls name end"
-*)
+  "cls \<le> cls2 \<Longrightarrow>
+   assoc_name |\<in>| fmdom assocs \<Longrightarrow>
+   fmlookup assocs assoc_name = Some assoc \<Longrightarrow>
+   fmlookup assoc role = Some end \<Longrightarrow>
+   from_role |\<in>| fmdom assoc \<Longrightarrow>
+   from_role \<noteq> role \<Longrightarrow>
+   fmlookup assoc from_role = Some from_end \<Longrightarrow>
+   assoc_end_class from_end = cls2 \<Longrightarrow>
+   find_association assocs cls role cls2 end"
 
-(*
-lemma find_association_code [code_pred_intro]:
-  "fmfilter (\<lambda>assoc.
-      case fmlookup assocs assoc of None \<Rightarrow> False | Some ends \<Rightarrow>
-        assoc_refer_class (fmdrop name ends) cls \<and> assoc_refer_role ends name) assocs = a1 \<Longrightarrow>
-   fmlookup a1 assoc = Some ends \<Longrightarrow>
-   assoc_refer_class (fmdrop name ends) cls \<Longrightarrow>
-   fmlookup ends name = Some end \<Longrightarrow>
-   find_association assocs cls name end"
-  by (metis (no_types, lifting) find_association.intros fmdom'_notD fmlookup_filter option.distinct(1))
-*)
+class object_model = semilattice_sup +
+  fixes attribute :: "'a \<Rightarrow> attr \<Rightarrow> 'a \<Rightarrow> 'a type \<Rightarrow> bool"
+
+(*** Code Setup *************************************************************)
+
+section \<open>Code Setup\<close>
+
+definition "attrs_ok_fun attrs \<equiv> \<nexists>\<C> \<D>.
+  \<C> < \<D> \<and>
+  (case (fmlookup attrs \<C>, fmlookup attrs \<D>)
+    of (Some attrs\<^sub>\<C>, Some attrs\<^sub>\<D>) \<Rightarrow>
+      fBex (fmdom attrs\<^sub>\<C>) (\<lambda>attr.
+        fmlookup attrs\<^sub>\<C> attr \<noteq> None \<and>
+        fmlookup attrs\<^sub>\<D> attr \<noteq> None)
+    | _ \<Rightarrow> False)"
+
+lemma attrs_ok_code [code_abbrev, simp]:
+  "attrs_ok_fun attrs = attrs_ok attrs"
+proof
+  show "attrs_ok_fun attrs \<Longrightarrow> attrs_ok attrs"
+    unfolding attrs_ok_fun_def attrs_ok_def option.case_eq_if
+    apply auto
+    by (smt fBexI fmdomI fmdom_notD fmdom_notI option.sel)
+  show "attrs_ok attrs \<Longrightarrow> attrs_ok_fun attrs"
+    unfolding attrs_ok_fun_def attrs_ok_def option.case_eq_if
+    by auto
+qed
+
+code_pred [show_modes] find_attribute .
+
+lemma fmember_code_predI [code_pred_intro]:
+  "Predicate_Compile.contains (fset xs) x \<Longrightarrow> x |\<in>| xs"
+  by (meson Predicate_Compile.containsE notin_fset)
+
+code_pred [show_modes] fmember
+  by (simp add: Predicate_Compile.containsI fmember.rep_eq)
+
+code_pred [show_modes] find_association .
 
 (*** Test Cases *************************************************************)
 
@@ -95,178 +121,15 @@ definition "attrs1 \<equiv> fmap_of_list [
     (STR ''cost'', Real[?])]),
   (Task, fmap_of_list [
     (STR ''description'', String[1])])]"
-(*
-lemma subclass1_code [code_pred_intro]:
-  "(cls :: classes1) \<le> cls"
-  "subclass1 cls cls2 \<Longrightarrow>
-   cls \<le> cls2"
-  by (simp_all add: less_classes1_def less_eq_classes1_def)
-*)
-(*
-lemma find_attribute_code [code_pred_intro]:
-  "fmlookup attrs cls = Some cls_attrs \<Longrightarrow>
-   fmlookup cls_attrs name = Some \<tau> \<Longrightarrow>
-   find_attribute attrs cls name cls \<tau>"
-  "subclass1 cls cls2 \<Longrightarrow>
-   fmlookup attrs cls2 = Some cls_attrs \<Longrightarrow>
-   fmlookup cls_attrs name = Some \<tau> \<Longrightarrow>
-   find_attribute attrs cls name cls2 \<tau>"
-  by (simp_all add: find_attribute.intros less_classes1_def less_eq_classes1_def)
-*)
-(*
-datatype ty = A | B | C
 
-inductive lty where
-  "lty A C"
-| "lty B C"
+value "attrs_ok attrs1"
 
-instantiation ty :: order
-begin
-
-definition "(<) \<equiv> lty"
-definition "x \<le> y \<equiv> x = y \<or> lty x y"
-
-instance
-  apply intro_classes
-  using less_eq_ty_def less_ty_def lty.simps by auto
-
-end
-
-inductive pred1 where
-  "x \<le> y \<Longrightarrow>
-   pred1 x y"
-
-lemma pred1_ty_code [code_pred_intro]:
-  "x = y \<Longrightarrow>
-   pred1 x y"
-  "lty x y \<Longrightarrow>
-   pred1 x y"
-  by (simp_all add: less_eq_ty_def pred1.intros r_into_rtranclp)
-
-code_pred [show_modes] pred1
-  using less_eq_ty_def pred1.simps by blast
-
-values "{x. pred1 A x}"
-
-
-inductive pred2 where
-  "pred1 x y \<Longrightarrow>
-   pred2 x y"
-
-(*
-lemma pred2_ty_code [code_pred_intro]:
-  "pred1 x y \<Longrightarrow>
-   pred2 x y"
-  by (simp_all add: pred1_ty_code pred2.intros)
-
-code_pred [show_modes] pred2
-  using pred2.cases by blast
-*)
-lemma pred2_ty_code [code_pred_intro]:
-  "x = y \<Longrightarrow>
-   pred2 x y"
-  "lty x y \<Longrightarrow>
-   pred2 x y"
-  by (simp_all add: pred1_ty_code pred2.intros)
-
-code_pred [show_modes] pred2
-  using less_eq_ty_def pred1.cases pred2.simps by blast
-
-values "{x. pred2 A x}"
-
-
-
-
-
-datatype ty = A | B | C | D
-
-inductive lty where
-  "lty A C"
-| "lty B C"
-| "lty C D"
-
-inductive_cases lty_x_A [elim!]: "lty x A"
-inductive_cases lty_x_B [elim!]: "lty x B"
-inductive_cases lty_x_C [elim!]: "lty x C"
-inductive_cases lty_x_D [elim!]: "lty x D"
-
-code_pred [show_modes] lty .
-
-instantiation ty :: order
-begin
-
-definition "(<) \<equiv> lty\<^sup>+\<^sup>+"
-definition "(\<le>) \<equiv> lty\<^sup>*\<^sup>*"
-
-lemma ty_less_le_not_le:
-  "x < y \<longleftrightarrow> x \<le> y \<and> \<not> (y \<le> x)"
-  for x y :: ty
-  unfolding less_ty_def less_eq_ty_def
-  apply auto
-  apply (metis Nitpick.rtranclp_unfold lty.cases lty_x_A lty_x_B lty_x_C tranclp.cases tranclpD)
-  by (metis rtranclpD)
-
-instance
-  apply intro_classes
-  apply (simp add: ty_less_le_not_le)
-  apply (simp add: less_eq_ty_def)
-  apply (metis less_eq_ty_def rtranclp_trans)
-  by (metis (mono_tags, lifting) less_eq_ty_def less_ty_def rtranclpD ty_less_le_not_le)
-
-end
-
-inductive pred1 where
-  "x \<le> y \<Longrightarrow>
-   pred1 x y"
-
-inductive pred2 where
-  "pred1 x y \<Longrightarrow>
-   pred2 x y"
-
-lemma pred1_ty_code [code_pred_intro]:
-  "x = y \<Longrightarrow>
-   pred1 x y"
-  "lty x y \<Longrightarrow>
-   pred1 x y"
-  by (simp_all add: less_eq_ty_def pred1.intros r_into_rtranclp)
-
-code_pred [show_modes] pred1
-  apply (erule pred1.cases)
-*)
-(*
-code_pred [show_modes] find_attribute
-  by (metis find_attribute.cases less_classes1_def less_eq_classes1_def)
-*)
-
-inductive find_attribute where
-  "cls \<le> cls2 \<Longrightarrow>
-   fmlookup attrs cls2 = Some cls_attrs \<Longrightarrow>
-   fmlookup cls_attrs name = Some \<tau> \<Longrightarrow>
-   find_attribute attrs cls name cls2 \<tau>"
-
-code_pred [show_modes] find_attribute .
-
-values "{(c, t). find_attribute attrs1 Employee (STR ''name'') c t}"
-values "{(c, t). find_attribute attrs1 Employee (STR ''position'') c t}"
-(*
-inductive elems where
-  "x |\<in>| xs \<Longrightarrow>
-   elems xs x"
-
-primrec elems_fun where
-  "elems_fun "
-
-term "set_of_pred"
-term subclass1_i_o
-value "set_of_pred (subclass1_i_o Employee)"
-
-code_pred [show_modes] elems .
-
-values "{x. elems {|1::nat,2,3|} x}"
-
-lemma find_assoc1_code [code_pred_intro]:
-  "find_assoc1 assocs (fmdom assocs)"
-*)
+lemma find_attribute_det:
+  "attrs_ok attrs \<Longrightarrow>
+   find_attribute attrs \<C> attr \<D> \<tau> \<Longrightarrow>
+   find_attribute attrs \<C> attr \<E> \<sigma> \<Longrightarrow>
+   \<D> = \<E> \<and> \<tau> = \<sigma>"
+  sorry
 
 definition assocs1 :: "classes1 assocs" where
   "assocs1 \<equiv> fmap_of_list [
@@ -294,227 +157,44 @@ definition assocs1 :: "classes1 assocs" where
     (STR ''tasks'', (Task, 0, 5)),
     (STR ''assignee'', (Employee, 0, 1))])]"
 
-lemma fmember_code_predI [code_pred_intro]:
-  "Predicate_Compile.contains (fset xs) x \<Longrightarrow> x |\<in>| xs"
-  by (meson Predicate_Compile.containsE notin_fset)
+instantiation classes1 :: object_model
+begin
 
-code_pred [show_modes] fmember
-  by (simp add: Predicate_Compile.containsI fmember.rep_eq)
+definition "attribute_classes1 = find_attribute attrs1"
 
-value "{x. x \<in> fmdom' assocs1}"
-values "{x. x |\<in>| fmdom assocs1}"
-(*
-inductive find_assoc where
-  "a |\<in>| fmdom assocs \<Longrightarrow>
-   fmlookup assocs a = Some assoc \<Longrightarrow>
-   fmlookup assoc name = Some end \<Longrightarrow>
-   find_assoc assocs cls name end"
+instance ..
 
-code_pred [show_modes] find_assoc .
-*)
-(*
-definition "fset_of_assocs assocs \<equiv>
-  ffold (\<lambda>(a, r, e) y. ffold (\<lambda>x z. finsert (a, r, x) z) fempty e) fempty
-    (fset_of_fmap (fmmap_keys (\<lambda>k v. (k, fset_of_fmap v)) assocs))"
-*)
-(*
-definition "sorted_list_of_assocs assocs \<equiv>
-  concat (fold (\<lambda>(a, r) y. (fold (\<lambda>x z. (a, x) # z) r []) # y)
-    (sorted_list_of_fmap (fmmap sorted_list_of_fmap assocs)) [])"
-*)
-(*
-primrec product_lists :: "'a list list \<Rightarrow> 'a list list" where
-"product_lists [] = [[]]" |
-"product_lists (xs # xss) = concat (map (\<lambda>x. map (Cons x) (product_lists xss)) xs)"
-*)
-(*
-value "sorted_list_of_fmap (fmmap (\<lambda>xm. map (\<lambda>x. fmdrop x xm) (sorted_list_of_fset (fmdom xm))) assocs)"
-term map
+end
 
-value "(sorted_list_of_fmap (fmmap (\<lambda>xm. map (\<lambda>x. sorted_list_of_fmap (fmdrop x xm)) (sorted_list_of_fset (fmdom xm))) assocs1))"
+print_theorems
 
-type_synonym 'a binary_assoc = "assoc \<times> role \<times> 'a assoc_end \<times> role \<times> 'a assoc_end"
+definition "model_ok m \<equiv> attrs_ok (fst m)"
 
-definition "from_role \<equiv> fst \<circ> snd"
-definition "from_assoc_end \<equiv> fst \<circ> snd \<circ> snd"
-definition "to_role \<equiv> fst \<circ> snd \<circ> snd \<circ> snd"
-definition "to_assoc_end \<equiv> snd \<circ> snd \<circ> snd \<circ> snd"
-
-definition sorted_list_of_assocs :: "'a assocs \<Rightarrow> 'a binary_assoc list" where
-  "sorted_list_of_assocs assocs \<equiv> concat (concat (
-    map (\<lambda>(assoc, roles).
-      map (\<lambda>(from, ends).
-        map (\<lambda>end. (assoc, end)) ends) roles)
-      (sorted_list_of_fmap (fmmap (\<lambda>xm.
-        (sorted_list_of_fmap (fmmap_keys (\<lambda>x v. map (\<lambda>y. (x, v, y))
-          (sorted_list_of_fmap (fmdrop x xm))) xm))) assocs))))"
-
-definition "roles xs \<equiv> map (\<lambda>assoc. (assoc_end_class (from_assoc_end assoc), assoc)) xs"
-
-value "roles (sorted_list_of_assocs assocs1)"
-value "sorted_list_of_assocs assocs1"
-*)
-(*
-definition "sorted_list_of_assocs assocs \<equiv>
-   (fold (\<lambda>(a, r) y. y @ [fold (\<lambda>(x, y) z. z @ [(a, y)]) r []])
-    (sorted_list_of_fmap (fmmap (\<lambda>xm.
-      sorted_list_of_fmap (fmmap_keys (\<lambda>x v. map (\<lambda>y. (x, v, y)) (sorted_list_of_fmap (fmdrop x xm)))
-          xm))
-      assocs)) [])"
-
-definition "sorted_list_of_assocs assocs \<equiv>
-   (fold (\<lambda>(a, r) y. y @ [fold (\<lambda>x z. z @ [(a, x)]) r []])
-    (sorted_list_of_fmap (fmmap (\<lambda>xm.
-      map (\<lambda>x. map (\<lambda>y. (x, y)) (sorted_list_of_fmap (fmdrop x xm)))
-          (sorted_list_of_fset (fmdom xm)))
-      assocs)) [])"
-*)
-(*
-value "let x = fmap_of_list [
-    (STR ''manages'', (Project, 0::nat, 2::nat)),
-    (STR ''manager'', (Employee, 1, 1))] in
-  map (\<lambda>x. (x, fmdrop x xm)) (sorted_list_of_fset (fmdom xm))"
-
-term "fmdrop"
-
-value "fmmap sorted_list_of_fmap assocs1"
-
-definition "sorted_list_of_assocs assocs \<equiv>
-   (fold (\<lambda>(a, r) y. y @ [fold (\<lambda>x z. z @ [(a, x)]) r []])
-    (sorted_list_of_fmap (fmmap sorted_list_of_fmap assocs)) [])"
-
-value "assocs1"
-
-term fmmap
-term "(fmmap_keys (\<lambda>k v. (k, sorted_list_of_fmap v)) assocs1)"
-term "(sorted_list_of_fmap (fmmap_keys (\<lambda>k v. (sorted_list_of_fmap v)) assocs1))"
-
-value "[[1::nat,2],[3,4,5],[6,7]]"
-(*
-value "fold (\<lambda>x y. product_lists [y,y]) [[1::nat,2],[3,4,5],[6,7]] ([] :: nat list)"
-*)
-value "product [[1::nat,2],[3,4,5],[6,7]]"
-term "product"
-value "subseqs [1::nat, 2, 3]"
-value "product_lists [[1::nat,2,3],[4,5,6]]"
-value "product_lists [[1::nat,2],[3,4,5],[6,7]]"
-value "List.n_lists 3 [1::nat,2,3]"
-
-(*
-primrec n_lists :: "nat \<Rightarrow> 'a list \<Rightarrow> 'a list list" where
-"n_lists 0 xs = [[]]" |
-"n_lists (Suc n) xs = concat (map (\<lambda>ys. map (\<lambda>y. y # ys) xs) (n_lists n xs))"
-*)
-(*
-primrec n_lists :: "'a list \<Rightarrow> ('a \<times> 'a) list" where
-"n_lists 0 xs = [[]]" |
-"n_lists (Suc n) xs = concat (map (\<lambda>ys. map (\<lambda>y. y # ys) xs) (n_lists n xs))"
-*)
-term filter
-value "n_lists 2 [1::nat,2,3]"
-value "shuffle [1::nat,2] [3,4]"
-
-primrec perm :: "'a list \<Rightarrow> 'a list \<Rightarrow> 'a list list" where
-  "perm xs [] = [xs]"
-| "perm xs (y # ys) = (perm (y # xs) ys)"
-
-value "perm ([] :: nat list) [1::nat,2,3]"
-
-term "fold (\<lambda>x y. y) [[1::nat,2],[3,4,5],[6,7]] []"
-value "fold (\<lambda>x y. fold (\<lambda>p q. (x, p) # q) x []) [[1::nat,2],[3,4,5],[6,7]] []"
-
-term "(fold (\<lambda>(a, r, e) y. (fold (\<lambda>x z. (a, r, x) # z) e []) # y)
-    (sorted_list_of_fmap (fmmap_keys (\<lambda>k v. (k, sorted_list_of_fmap v)) assocs1)) [])"
-
-term "sorted_list_of_assocs assocs1"
-term sorted_list_of_fmap
-term prod
-
-value "sorted_list_of_assocs assocs1"
-
-term "ffold (\<lambda>(a, r, e) y. ffold (\<lambda>x z. finsert (a, r, x) z) fempty e) fempty
-  (fset_of_fmap (fmmap_keys (\<lambda>k v. (k, fset_of_fmap v)) assocs1))"
-
-term "fset_of_fmap (fmmap_keys (\<lambda>k v. (k, fset_of_fmap v)) assocs1)"
-*)
-(*
-inductive find_assoc where
-  "a |\<in>| fmdom assocs \<Longrightarrow>
-   fmlookup assocs a = Some assoc \<Longrightarrow>
-   fmlookup assoc name = Some end \<Longrightarrow>
-   find_assoc assocs cls name end"
-*)
-(*
-inductive find_association where
-  "cls \<le> cls2 \<Longrightarrow>
-   find_assoc_end assocs cls2 name = Some end \<Longrightarrow>
-   find_association assocs cls name cls2 end"
-
-lemma find_association_code [code_pred_intro]:
-  "find_assoc_end assocs cls name = Some end \<Longrightarrow>
-   find_association assocs cls name cls end"
-  "subclass1 cls cls2 \<Longrightarrow>
-   find_assoc_end assocs cls2 name = Some end \<Longrightarrow>
-   find_association assocs cls name cls2 end"
-  by (simp_all add: find_association.intros less_eq_classes1_def less_classes1_def)
-
-code_pred [show_modes] find_association
-  by (metis find_association.cases less_classes1_def less_eq_classes1_def)
-*)
-
-(*
-definition find_assocs :: "'a assocs \<Rightarrow> 'a \<Rightarrow> role \<Rightarrow> 'a assocs" where
-  "find_assocs assocs cls role \<equiv>
-    fmfilter (\<lambda>assoc.
-      case fmlookup assocs assoc of None \<Rightarrow> False | Some ends \<Rightarrow>
-        assoc_refer_class (fmdrop role ends) cls \<and> assoc_refer_role ends role) assocs"
-
-definition find_assoc_end :: "'a assocs \<Rightarrow> 'a \<Rightarrow> role \<Rightarrow> 'a assoc_end option" where
-  "find_assoc_end assocs cls role \<equiv>
-    let found = fmran (find_assocs assocs cls role) in
-    if fcard found = 1 then fmlookup (fthe_elem found) role else None"
-*)
-
-inductive find_association where
-  "cls \<le> cls2 \<Longrightarrow>
-   assoc_name |\<in>| fmdom assocs \<Longrightarrow>
-   fmlookup assocs assoc_name = Some assoc \<Longrightarrow>
-   fmlookup assoc name = Some end \<Longrightarrow>
-(*   find_assoc_end assocs cls2 name = Some end \<Longrightarrow>*)
-   find_association assocs cls name cls2 end"
-
-code_pred [show_modes] find_association .
-
-values "{(c, e). find_association assocs1 Employee STR ''projects'' c e}"
-values "{(c, e). find_association assocs1 Customer STR ''projects'' c e}"
-values "{(c, e). find_association assocs1 Project STR ''manager1'' c e}"
-
-value "find_assocs assocs1 Project STR ''manager''"
-value "find_assocs assocs1 Employee STR ''tasks''"
-value "find_assoc_end assocs1 Project STR ''manager''"
-value "find_assoc_end assocs1 Employee STR ''tasks''"
-
-value "find_assocs assocs1 Project STR ''manager1''"
-value "find_assoc_end assocs1 Project STR ''manager1''"
+typedef (overloaded) 'a good_model = "{m :: ('a :: ord) model. model_ok m}"
+proof -
+  have "model_ok (fmempty, fmempty)"
+    unfolding model_ok_def attrs_ok_def
+    by auto
+  thus ?thesis
+    by auto
+qed
 
 
-
-
-
-
+term attribute_classes1
+term "classes1.attribute"
 
 definition "model1 \<equiv> (attrs1, assocs1)"
 
 subsection \<open>Positive Cases\<close>
 
-value "find_assocs assocs1 Project STR ''manager''"
-value "find_assocs assocs1 Employee STR ''tasks''"
-value "find_assoc_end assocs1 Project STR ''manager''"
-value "find_assoc_end assocs1 Employee STR ''tasks''"
+values "{(c, t). attribute Employee (STR ''name'') c t}"
+values "{(c, t). find_attribute attrs1 Employee (STR ''name'') c t}"
+values "{(c, t). find_attribute attrs1 Employee (STR ''position'') c t}"
+values "{(c, e). find_association assocs1 Employee STR ''projects'' c e}"
+values "{(c, e). find_association assocs1 Customer STR ''projects'' c e}"
 
 subsection \<open>Negative Cases\<close>
 
-value "find_assocs assocs1 Project STR ''manager1''"
-value "find_assoc_end assocs1 Project STR ''manager1''"
+values "{(c, e). find_association assocs1 Project STR ''manager1'' c e}"
 
 end
